Risc0/Cirgen/Get.lean
@@ -1,70 +1,216 @@
 import Risc0.State.Defs
 import Risc0.State.Notation
+import Risc0.State.Set
+import Risc0.Cirgen.Defs
 
 namespace Risc0
 
-  def isGetValid (st : State) (buf : BufferVar) (back : Back) (offset : ℕ) :=
-    back ≤ st.cycle ∧
-    buf ∈ st.vars ∧
-    offset < st.bufferWidths[buf].get! ∧
-    (Buffer.back st buf back offset).isSome
+  section isGetValid
+    lemma isGetValid_def :
+      isGetValid st buf back offset = 
+      (back ≤ st.cycle ∧
+      buf ∈ st.vars ∧
+      offset < st.bufferWidths[buf].get! ∧
+      (Buffer.back st buf back offset).isSome) := rfl
 
-  lemma isGetValid_def :
-    isGetValid st buf back offset = 
-    (back ≤ st.cycle ∧
-    buf ∈ st.vars ∧
-    offset < st.bufferWidths[buf].get! ∧
-    (Buffer.back st buf back offset).isSome) := rfl
+    lemma isGetValid_set_of_ne (h : buf ≠ buf') :
+      isGetValid (State.set! st buf' index x) buf back offset = 
+      isGetValid st buf back offset := by
+      unfold isGetValid Buffer.back Back.toNat
+      simp
+      rw [State.set!_bufferWidths_get_of_ne h, State.set!_buffers_get_of_ne h]
+      aesop
+  end isGetValid
 
-  instance : Decidable (isGetValid st buf back offset) := by unfold isGetValid; exact inferInstance
+  section getImpl
+    lemma getImpl_def : getImpl st buf back offset = 
+      if isGetValid st buf back offset
+      then Option.some <| Lit.Val (Buffer.back st buf back offset).get!
+      else .none := rfl
 
-  def getImpl (st : State) (buf : BufferVar) (back : Back) (offset : ℕ) :=
-    if isGetValid st buf back offset
-    then Option.some <| Lit.Val (Buffer.back st buf back offset).get!
-    else .none
-
-  lemma getImpl_def : getImpl st buf back offset = 
-                      if isGetValid st buf back offset
-                      then Option.some <| Lit.Val (Buffer.back st buf back offset).get!
-                      else .none := rfl
-
-  --Review: should any of these be simps?
-  lemma getImpl_none_or_val : getImpl st buf back offset = .none ∨ ∃ x, getImpl st buf back offset = some (.Val x) := by
-    simp [getImpl]
-    aesop
-
-  lemma getImpl_val_of_some : getImpl st buf back offset = some lit → ∃ x, lit = .Val x := by
-    have h: getImpl st buf back offset = .none ∨ ∃ x, getImpl st buf back offset = some (.Val x) := getImpl_none_or_val
-    aesop
-
-  @[simp]
-  lemma getImpl_skip_none_update : getImpl (st[name] ←ₛ .none) buf back offset = getImpl st buf back offset := by
-    simp [State.update, getImpl, isGetValid, Buffer.back]
-
-  @[simp]
-  lemma getImpl_skip_val_update : getImpl (st[name] ←ₛ .some (.Val x)) buf back offset = getImpl st buf back offset := by
-    simp [State.update, getImpl, isGetValid, Buffer.back]
-
-  @[simp]
-  lemma getImpl_skip_get_update:
-    getImpl (st[name] ←ₛ getImpl st' buf' back' offset') buf back offset =
-    getImpl st buf back offset := by
-    generalize eq: getImpl st' buf' back' offset' = x
-    cases x with
-    | none => exact getImpl_skip_none_update
-    | some lit =>
-      have h: ∃ x, lit = Lit.Val x := getImpl_val_of_some eq
+    --Review: should any of these be simps?
+    lemma getImpl_none_or_val : getImpl st buf back offset = .none ∨ ∃ x, getImpl st buf back offset = some (.Val x) := by
+      simp [getImpl]
       aesop
 
-  lemma getImpl_skip_set_offset (h: offset ≠ offset'):
-    getImpl (State.set! st buf offset val) buf back offset' =
-    getImpl st buf back offset' := by
-      sorry
+    lemma getImpl_val_of_some : getImpl st buf back offset = some lit → ∃ x, lit = .Val x := by
+      have h: getImpl st buf back offset = .none ∨ ∃ x, getImpl st buf back offset = some (.Val x) := getImpl_none_or_val
+      aesop
 
-  @[simp]
-  lemma getImpl_dropFelts : 
-    getImpl (State.dropFelts st y) buf back offset = getImpl st buf back offset := by
-    unfold State.dropFelts getImpl
-    aesop
+    @[simp]
+    lemma getImpl_skip_none_update : getImpl (st[name] ←ₛ .none) buf back offset = getImpl st buf back offset := by
+      simp [State.update, getImpl, isGetValid, Buffer.back]
+
+    @[simp]
+    lemma getImpl_skip_val_update : getImpl (st[name] ←ₛ .some (.Val x)) buf back offset = getImpl st buf back offset := by
+      simp [State.update, getImpl, isGetValid, Buffer.back]
+
+    @[simp]
+    lemma getImpl_skip_get_update:
+      getImpl (st[name] ←ₛ getImpl st' buf' back' offset') buf back offset =
+      getImpl st buf back offset := by
+      generalize eq: getImpl st' buf' back' offset' = x
+      cases x with
+      | none => exact getImpl_skip_none_update
+      | some lit =>
+        have h: ∃ x, lit = Lit.Val x := getImpl_val_of_some eq
+        aesop
+
+    @[simp]
+    lemma getImpl_dropFelts : 
+      getImpl (State.dropFelts st y) buf back offset = getImpl st buf back offset := by
+      unfold State.dropFelts getImpl
+      aesop
+
+    lemma getImpl_skip_set (h : buf ≠ buf') :
+      getImpl (State.set! st buf' index x) buf back offset = getImpl st buf back offset := by
+      unfold getImpl Buffer.back Buffer.get! Buffer.Idx.time Buffer.Idx.data Back.toNat
+      simp [isGetValid_set_of_ne h]
+      rw [State.get!_set!_of_ne h]
+
+    lemma getImpl_skip_set_offset_of_none_aux (h : st.buffers[buf] = none) : State.set! st buf a b =
+                                            {st with buffers := st.buffers[buf] ←ₘ []} := by
+      unfold State.set!; simp [h]
+      unfold State.setBufferElementImpl; simp [Option.get!, h]
+      simp [panicWithPosWithDecl, panic, panicCore, default, instInhabitedList]
+      unfold Buffer.set?
+      simp
+
+    lemma getImpl_skip_set_offset_of_none (contra : st.buffers[buf] = none) :
+      getImpl (State.set! st buf offset val) buf back offset' =
+      getImpl st buf back offset' := by
+      rw [getImpl_skip_set_offset_of_none_aux contra]
+      simp [getImpl, isGetValid, Buffer.back]
+      rw [contra]
+      simp [Option.get!, panicWithPosWithDecl, panic, panicCore, default]
+
+    private lemma getImpl_skip_set_offset_of_some_aux {st : State}
+      (h : List.get! (List.get! buffer (List.length buffer - (1 : ℕ))) offset = some val)
+      (h₁ : st.buffers buf = some buffer) :
+      getImpl (State.set! st buf offset val) buf back offset' = getImpl st buf back offset' := by
+        simp [
+            State.set!, State.setBufferElementImpl, Buffer.set?, Buffer.getBufferAtTime!, Buffer.Idx.time, Buffer.Idx.data,
+            getElem
+        ]
+        simp [h₁, h, Option.isEqSome]
+        congr
+        unfold Map.update; funext z
+        have : State.buffers st z = st.buffers[z] := rfl; rw [this]
+        aesop
+
+    lemma List.get!_set {α : Type} [Inhabited α] {l : List α} {i : ℕ} {v : α} (h : i < l.length) :
+      List.get! (List.set l i v) i = v := by
+      induction l generalizing i with
+        | nil => cases h
+        | cons hd tl ih =>
+          cases i with
+            | zero => aesop
+            | succ i => simp at h
+                        have : i < tl.length := Nat.lt_of_succ_lt_succ h
+                        rw [←ih this]
+                        aesop
+
+    lemma List.get!_set_of_ne {α : Type} [Inhabited α] {l : List α} {i i' : ℕ} {v : α}
+      (h : i < l.length) (h₁ : i ≠ i') : List.get! (List.set l i v) i' = List.get! l i' := by
+      induction l generalizing i i' with
+        | nil => cases h
+        | cons hd tl ih =>
+          cases i <;> cases i' <;> aesop
+          have : n < tl.length := Nat.lt_of_succ_lt_succ h
+          rw [ih this h₁]
+
+    private lemma getImpl_skip_set_offset_of_some_aux'_aux
+      (h₀ : offset ≠ offset')
+      (h : lastIdx = List.length buffer - (1 : ℕ))
+      (h₁ : lastRow = List.get! buffer lastIdx)
+      (h₂ : st.buffers[buf] = some buffer) :
+      isGetValid
+        { buffers := st.buffers[buf] ←ₘ List.set buffer lastIdx (List.set lastRow offset (some val)),
+          bufferWidths := st.bufferWidths, constraints := st.constraints, cycle := st.cycle, felts := st.felts,
+          isFailed := st.isFailed, props := st.props, vars := st.vars } buf back offset' ↔
+      isGetValid st buf back offset' := by
+      subst h h₁ 
+      unfold isGetValid
+      simp [Buffer.back, Buffer.get!, Buffer.Idx.data, Buffer.Idx.time]
+      aesop <;>
+        generalize eq : List.length buffer - (1 : ℕ) = lastIdx at * <;>
+        generalize eq₁ : List.get! buffer lastIdx = lastRow at * <;>
+        generalize eq₂ : st.cycle - Back.toNat back = cycleIdx at *
+      · rw [Option.isSome_iff_exists] at a_3 ⊢
+        rcases a_3 with ⟨w₃, h₃⟩; use w₃
+        by_cases eq₃ : cycleIdx = lastIdx
+        · subst eq₃
+          rw [List.get!_set, List.get!_set_of_ne _ h₀] at h₃; rw [eq₁]; exact h₃
+          sorry; sorry
+        · rw [List.get!_set_of_ne _ (Ne.symm eq₃)] at h₃; exact h₃
+          sorry
+      · rw [Option.isSome_iff_exists] at a_3 ⊢
+        rcases a_3 with ⟨w₃, h₃⟩; use w₃
+        by_cases eq₃ : cycleIdx = lastIdx
+        · subst eq₃
+          rw [List.get!_set, List.get!_set_of_ne _ h₀]; aesop
+          sorry; sorry
+        · rw [List.get!_set_of_ne _ (Ne.symm eq₃)]; exact h₃
+          sorry
+
+    private lemma getImpl_skip_set_offset_of_some_aux' {st : State}
+      (h₀ : offset ≠ offset')
+      (h : List.get! (List.get! buffer (List.length buffer - (1 : ℕ))) offset ≠ some val)
+      (h₁ : st.buffers buf = some buffer) :
+      getImpl (State.set! st buf offset val) buf back offset' = getImpl st buf back offset' := by
+        generalize eq : List.length buffer - (1 : ℕ) = lastIdx at *
+        have : State.buffers st buf = st.buffers[buf] := rfl; rw [this] at h₁
+        simp [
+          State.set!, State.setBufferElementImpl, Buffer.set?, Buffer.getBufferAtTime!, Buffer.Idx.time, Buffer.Idx.data
+        ]
+        simp only [h₁, Option.get!_of_some, ge_iff_le, tsub_eq_zero_iff_le, eq]
+        generalize eq₁ : List.get! buffer lastIdx = lastRow
+        by_cases eq₂ : (List.get! lastRow offset).isNone <;> simp [eq₂]
+        · have :
+            Option.isEqSome (List.get! lastRow offset) val = false := by
+            simp [Option.isEqSome]
+            generalize eq₃ : List.get! lastRow offset = elem at *
+            aesop
+          simp only [this, ite_false]
+          unfold getImpl
+          congr 1
+          · rw [getImpl_skip_set_offset_of_some_aux'_aux h₀] <;> simp [*]
+          · simp [Buffer.back, Buffer.get!, Buffer.Idx.time, Buffer.Idx.data, h₁]
+            generalize eq₃ : st.cycle - Back.toNat back = cycleIdx
+            by_cases eq₄ : cycleIdx = lastIdx
+            · subst eq₄
+              rw [List.get!_set, List.get!_set_of_ne _ h₀, ←eq₁]
+              sorry; sorry
+            · rw [List.get!_set_of_ne _ (Ne.symm eq₄)]
+              sorry
+        · have :
+            Option.isEqSome (List.get! lastRow offset) val = false := by
+            simp [Option.isEqSome]
+            generalize eq₃ : List.get! lastRow offset = elem at *
+            aesop
+          simp [this]
+          rfl
+
+    lemma getImpl_skip_set_offset_of_some (h : offset ≠ offset') (h₁ : st.buffers[buf].isSome) :
+      getImpl (State.set! st buf offset val) buf back offset' =
+      getImpl st buf back offset' := by
+        rw [Option.isSome_iff_exists] at h₁
+        rcases h₁ with ⟨buffer, h₁⟩
+        let lastIdx := buffer.length - 1
+        by_cases eq₁ : List.get! (List.get! buffer lastIdx) offset = val
+        · exact getImpl_skip_set_offset_of_some_aux eq₁ h₁
+        · exact getImpl_skip_set_offset_of_some_aux' h eq₁ h₁
+
+    lemma getImpl_skip_set_offset (h: offset ≠ offset') :
+      getImpl (State.set! st buf offset val) buf back offset' =
+      getImpl st buf back offset' := by
+      by_cases eq : st.buffers[buf].isNone
+      · rw [Option.isNone_iff_eq_none] at eq
+        rw [getImpl_skip_set_offset_of_none eq]
+      · have : st.buffers[buf].isSome := by
+          rwa [Option.isNone_iff_eq_none, ←ne_eq, Option.ne_none_iff_isSome] at eq
+        rw [getImpl_skip_set_offset_of_some h this]
+  end getImpl
+
 
 end Risc0
