Risc0/State/DropFelts.lean
@@ -1,6 +1,7 @@
 import Risc0.State.Defs
 import Risc0.Cirgen.Defs
 import Risc0.State.Notation
+import Risc0.State.Update
 
 namespace Risc0.State
 
@@ -43,10 +44,9 @@ namespace Risc0.State
       ((State.dropFelts st y)[k] ←ₛ getImpl st buf back offset) =
       State.dropFelts (st[k] ←ₛ getImpl st buf back offset) y := by
       unfold State.dropFelts getImpl
-      aesop
-      simp [State.updateFelts, Map.drop, Map.update]
-      funext z
-      aesop
+      by_cases h_isGetValid: (isGetValid st buf back offset)
+      . simp only [h_isGetValid, ite_true, update_val', updateFelts, ne_eq, h, not_false_eq_true, Map.update_drop_swap]
+      . simp only [update, h_isGetValid, ite_false]
   end GetImpl
 
   -- Naughty
