Risc0/State/Set.lean
@@ -1,11 +1,56 @@
 import Risc0.State.Defs
+import Risc0.State.Notation
+import Risc0.Cirgen.Defs
 
 namespace Risc0.State
 
-@[simp]
-lemma set!_felts {st : State} {bufferVar : BufferVar} {offset : ℕ} {val : Felt} :
-  (st.set! bufferVar offset val).felts = st.felts := by
-  unfold set! setBufferElementImpl
-  aesop
+  section MemberAccess
+    @[simp]
+    lemma set!_felts {st : State} {bufferVar : BufferVar} {offset : ℕ} {val : Felt} :
+      (st.set! bufferVar offset val).felts = st.felts := by
+      unfold set! setBufferElementImpl
+      aesop
+
+    @[simp]
+    lemma set!_cycle {st : State} : (st.set! buf off x).cycle = st.cycle := by
+      unfold set! setBufferElementImpl
+      aesop
+
+    @[simp]
+    lemma set!_vars {st : State} : (st.set! buf off x).vars = st.vars := by
+      unfold set! setBufferElementImpl
+      aesop
+  end MemberAccess
+
+  lemma set!_bufferWidths_get_of_ne {st : State} (h : buf ≠ buf') :
+    (st.set! buf' index x).bufferWidths[buf] = st.bufferWidths[buf] := by
+    unfold set! setBufferElementImpl
+    aesop
+
+  lemma set!_buffers_get_of_ne {st : State} (h : buf ≠ buf') : 
+    (st.set! buf' index x).buffers[buf] = st.buffers[buf] := by
+    unfold set! setBufferElementImpl Map.update
+    rw [Map.getElem_def]
+    aesop
+
+  lemma set!_get_getImpl_comm {st : State} : 
+    (st[x] ←ₛ getImpl st buf back offset).set! buf' index y =
+    (State.set! st buf' index y)[x] ←ₛ getImpl st buf back offset := by
+    unfold State.update getImpl
+    aesop <;> unfold set! setBufferElementImpl <;> aesop
+
+  -- TODO rename get_set!_of_ne?
+  lemma get!_set!_of_ne (h : buf ≠ buf') :
+    (State.set! st buf' index x).buffers[buf] = st.buffers[buf] := by
+    unfold State.set! State.setBufferElementImpl Map.update
+    rw [Map.getElem_def]
+    aesop
+
+  @[simp]
+  lemma get_set!_getElem {st : State} :
+    (State.set! st buf offset val).bufferWidths[buf] =
+    st.bufferWidths[buf] := by
+    unfold State.set! State.setBufferElementImpl
+    aesop
 
 end Risc0.State
